![Image](https://pic4.zhimg.com/80/v2-fce1ed903c44794d7d56adc837b5e66c.jpg)

# 代数拓扑Algebraic topology笔记整理 第一章 奇异同调 

## §2 Chain complexes and chain mappings 

### 2.1 Chain complexes and homology groups 

$\bf Def\ 2.1\text{ (chain complex)}$

A chain complex(链复形) $C=(C_q,\partial_q)$ consists of a sequence of Abelian groups $\{C_q\}$ with homomorphisms $\{\partial_q:C_q\to C_{q-1}\}$ satisfying $\partial_q\circ\partial_{q+1}=0$ , called boundary mappings(边缘映射).

$$\begin{CD}
\cdots
@>\partial_{q+2}>> C_{q+1}
@>\partial_{q+1}>> C_q
@>\partial_{q}>>
\cdots
\end{CD}$$

<br/><br/>

$\bf Def\ 2.2\text{ (homology group)}$

$Z_q=\mathrm{Ker}(\partial_q)\subset C_q$ is called a group of cycles(闭链群), $B_q=\mathrm{Im}(\partial_{q+1})\subset C_q$ is called a group of boundaries(边缘链群). $\forall c_q\in B_q,\exists c_{q+1}\in C_{q+1}$ s.t. $c_q=\partial_{q+1}(c_{q+1})$ , then $\partial_{q}(c_q)=\partial_{q}\partial_{q+1}(c_{q+1})=0\Rightarrow c_q\in Z_q\Rightarrow B_q\subset Z_q$ . The homology group(同调群) is $H_q=Z_q/B_q$ . We sometimes use notations $Z_\ast=\{Z_q\}$ , $B_\ast=\{B_q\}$ , $H_\ast=\{H_q\}$ .

$\bf Rmk$

Since $C_q$ is Abelian, we obtain $B_q\lhd Z_q$ is normal, therefore $H_q$ is an Abelian group. $[\tilde z_q]=[z_q]\in H_q\Leftrightarrow\tilde z_q-z_q\in B_q$ .

<br/><br/>

### 2.2 Chain mappings and its induced homomorphism 

$\bf Def\ 2.3\text{ (chain mapping)}$

A chain mapping(链映射) $f:C\to D$ between C and D is a sequence of homomorphisms $\{f_q:C_q\to D_q\}$ s.t. the following diagram commutes, i.e. $f_q\circ\partial_{q+1}=\partial_{q+1}\circ f_{q+1}$ .

$$
\begin{CD}
\cdots
@>\partial_{q+2}>> C_{q+1}
@>\partial_{q+1}>> C_{q}
@>\partial_{q}>> C_{q-1}
@>\partial_{q-1}>> \cdots\\
@. @V f_{q+1} VV @Vf_{q}VV @Vf_{q-1}VV @.\\
\cdots
@>\partial_{q+2}>> D_{q+1}
@>\partial_{q+1}>> D_{q}
@>\partial_{q}>> D_{q-1}
@>\partial_{q-1}>> \cdots\\
\end{CD}$$

$\bf Rmk$

Given two chain mappings $f:C\to D,g:D\to E$ , from $g_qf_q\partial_{q+1}=\partial_{q+1}g_{q+1}f_{q+1}$ we know $g\circ f:C\to E$ is a chain mapping. Therefore $\{\text{chain complex, chain mapping}\}$ is a category, called the category of chain complexes(链复形的范畴).

<br/><br/>

$\bf Prop\ 2.4$

A chain mapping $f:C\to D$ induces homomorphisms $f_\ast=\{f_{\ast q}:H_q(C)\to H_q(D)\}$ between homology groups, where $f_{\ast q}([z_q])=[f_q(z_q)]$ .

> $\it Proof$
>  
> 1. Check: $[f_q(z_q)]\in H_q(D)$
>  
> $$
> \begin{aligned}
> &\partial_q f_q(z_q)=f_{q-1}\partial_q(z_q)=0\\
> \Rightarrow& f_q(z_q)\in Z_q(D)\\
> \Rightarrow& [f_q(z_q)]\in H_q(D)
> \end{aligned}
> $$
>  
> 2. Check: $f_{\ast q}$ is well-defined, i.e. $f_{\ast q}$ is independent of choices of $z_q\in[z_q]\in H_q(C)$ 
>  
> Assume $\tilde z_q\in Z_q$ s.t. $[\tilde z_q]=[z_q]\Leftrightarrow\tilde z_q-z_q\in B_q$ , then $\exists c_{q+1}\in C_{q+1}$ s.t. $\tilde z_q-z_q=\partial_{q+1}(c_{q+1})$ . $f_q(\tilde z_q)-f_q(z_q)=f_q(\tilde z_q-z_q)=f_q\partial_{q+1}(c_{q+1})=\partial_{q+1}f_{q+1}(c_{q+1})\in B_{q}(D)$ . Therefore $[f_q(z_q)]=[f_q(\tilde z_q)]$ .
>  
> 3. Check: $f_{\ast q}$ is a homomorphism
>  
> $$\begin{aligned}
> &f_{\ast q}([z_q])+f_{\ast q}([z'_q])=[f_q(z_q)]+[f_q(z'_q)]\\
> =&[f_q(z_q)+f_q(z'_q)]=[f_{q}(z_q+z'_q)]\\
> =&f_{\ast q}([z_q+z'_q])=f_{\ast q}([z_q]+[z'_q])
> \end{aligned}
> $$

$\bf Rmk$

Given two chain mappings $f:C\to D,g:D\to E$ , we have $(gf)_\ast=g_\ast f_\ast$ .

<br/><br/>

### 2.3 Chain homotopy 

How to construct properly 'isomorphic relation' between two chain complexes?

Recall:
1. Two continuous maps $f,g:X\to Y$ (topological spaces) are homotopic(同伦的) if there exists a continuous map $G:X\times[0,1]\to Y$ s.t. $G(x,0)=f(x)$ and $G(x,1)=g(x)$ ;
2. Two topological spaces $X,Y$ are homotopy equivalent(同伦等价的) if there exists continuous mappings $f:X\to Y$ and $g:Y\to X$ s.t. $g\circ f\sim\mathrm{id}_X$ and $f\circ g\sim\mathrm{id}_Y$ .

<br/><br/>

We hope it satisfies $f_\ast=g_\ast:H_\ast(C)\to H_\ast(D)$ for two 'isomorphic' chain mappings $f,g:C\to D$ . To achieve $f_{\ast q}=g_{\ast q}$ , we need $[f_{q}(z_q)]=[g_{q}(z_q)]$ , i.e. $g_q(z_q)-f_q(z_q)\in B_q(D)$ , i.e. $\exists d_{q+1}\in D_{q+1}$ s.t. $g_q(z_q)-f_q(z_q)=\partial_{q+1}(d_{q+1})$ . Note that both $f_q,g_q$ are mappings from $C_q\to D_q$ while $\partial_{q+1}:D_{q+1}\to D_q$ . We hope to find a group homomorphism $T_q:C_q\to D_{q+1}$ where $d_{q+1}=T_q(z_q)$ . Also notice that $\partial_{q}(z_q)=0$ , therefore we have $g_q(z_q)-f_q(z_q)=\partial_{q+1}T_{q}(z_q)+T_{q-1}\partial_{q}(z_q)$ . In this case, the right-hand side $\partial_{q+1}T_{q}+T_{q-1}\partial_{q}$ is a mapping from $C_q\to D_q$ .

<br/><br/>

$\bf Def\ 2.5\text{ (chain homotopy)}$

Two chain mappings $f,g:C\to D$ are chain homotopic(链同伦的) if there exists homomorphisms $T=\{T_q:C_q\to D_{q+1}\}$ s.t. $g_q-f_q=\partial_{q+1}T_{q}+T_{q-1}\partial_{q}$ , denoted by $T:f\simeq g:C\to D$ . $T$ is called a chain homotopy(链同伦).

$\bf Thm\ 2.6$

Two chain mappings $f\simeq g:C\to D$ induce the same homomorphisms $f_\ast=g_\ast:H_\ast(C)\to H_\ast(D)$ if they are chain homotopic.

$\bf Prop\ 2.7$

Chain homotopy between chain mappings is an equivalence relation, i.e. For any $f,g,h:C\to D$ , we have
1. $f\simeq f$ (choose $\tilde{T}=0$ );
2. $f\simeq g\Rightarrow g\simeq f$ (choose $\tilde{T}=-T_q$ );
3. $f\simeq g,g\simeq h\Rightarrow f\simeq h$ (choose $\tilde{T}=T+T'$ ).

<br/><br/>

$\bf Prop\ 2.8$

Assume $f\simeq f':C\to D$ and $g\simeq g':D\to E$ , then $f\circ g\simeq f'\circ g'$ .

$\bf Rmk$

From the proof we will know the reason why we need $f\simeq g:C\to D$ to be $g_q-f_q=\partial_{q+1}T_{q}+T_{q-1}\partial_{q}$ but not $g_q-f_q=\partial_{q+1}T_{q}$ .

<br/><br/>

$\bf Def\ 2.9\text{ (chain homotopy equivalent)}$

Two chain complexes $C$ and $D$ are chain homotopy equivalent(链同伦等价的) if there exists chain mappings $f:C\to D,g:D\to C$ such that $g\circ f\simeq\mathrm{id}_C:C\to C,f\circ g\simeq\mathrm{id}_D:D\to D$ , denoted by $C\simeq D$ . $f$ and $g$ are both called chain homotopy equivalence.

$\bf Thm\ 2.10$

Two chain complexes have isomorphic homology groups if they are chain homotopy equivalent.

> $\it Proof$
>  
> From the view of mapping, $g_{\ast}\circ f_{\ast}=\mathrm{id}_{H_\ast(C)}$ and $f_{\ast}\circ g_{\ast}=\mathrm{id}_{H_\ast(D)}$ indicate that both $f_{\ast}$ and $g_{\ast}$ are bijective and thus $f_{\ast}:H_\ast(C)\to H_\ast(D)$ are group isomorphisms.

$\bf Prop\ 2.11$

Chain homotopy equivalence is an equivalence relation.

---

## §3 Singular homology groups

### 3.1 Singular simplices

$\bf Def\ 3.1\text{ (standard simplex)}$

A standard $q$-simplex(标准单形) is $\Delta_q=\{(x_0,x_1,\dots,x_q)\in\mathbb R^{n+1}:0\leq x_i\leq 1,\sum_{i=0}^q x_i=1\}$ , the vertexes(顶点) of $\Delta_q$ are $e_0=(1,0,\dots,0)$ , $e_1=(0,1,\dots,0)$ ... and $e_q=(0,0,\dots,1)$ .

![标准单形示意图](https://pica.zhimg.com/v2-785d256e76f58373f5f171894b12d122_720w.jpg?source=d16d100b)

<br/><br/>

$\bf Def\ 3.2\text{ (singular simplex)}$

A singular $q$-simplex(奇异单形) in topological space $X$ is a continuous mapping $\sigma:\Delta_q\to X$ 

$\bf e.g.$

Given a convex set(凸集) $C$ in Euclidean space and $c_0,c_1,\dots,c_q\in C$ , then there is a unique linear singular simplex(线性奇异单形) $(c_0c_1\dots c_q):\Delta_q\to C$ where $\sum_{i=0}^q x_ie_i\mapsto \sum_{i=0}^q x_ic_i$ . In particular, $\mathrm{id}_{\Delta_q}=(e_0e_1\dots e_q)$ .

<br/><br/>

### 3.2 Singular chain complexes and singular homology groups

In this section, we assume $X$ is a topological space.

$\bf Def\ 3.3\text{ (groups of singular chains)}$

The basis consists of all the $q$-singular simplices on $X$ generates a free Abelian group $S_q(X)$ , i.e. $\forall c_q\in S_q(X)$ , $\exists k_i\in\mathbb Z$ and singular simplices $\sigma_q^{(i)}:\Delta_q\to X$ in the basis such that $c_q=\sum_{i=1}^r k_i\sigma_q^{(i)}$ . $S_q(X)$ is called a group of singular chains(奇异链群) on $X$ , whose elements are singular chains(奇异链). We also define the group of singular chains of negative dimension to be zero $0$ .

<br/><br/>

Now we are going to define properly boundary mappings $\partial_q:S_q(X)\to S_{q-1}(X)$ such that $S_\ast(X)=(S_q(X),\partial_q)$ is a chain complex, i.e. we need $\partial_{q-1}\partial_q=0$ .

$\bf Def\ 3.4$

Given a singular simplex $\sigma_q:\Delta_q\to X$ , its boundary is defined as $\partial_q(\sigma_q)=\sum_{i=0}^q(-1)^i\sigma_q\circ(e_0\dots\hat e_i\dots e_q)$ . For any $c_q=\sum_{i=1}^r k_i\sigma_q^{(i)}\in S_q(X)$ , its boundary is defined as $\partial_q(c_q)=\sum_{i=1}^r k_i\partial_q(\sigma_q^{(i)})$ . One can easily prove $\partial_q:S_q(X)\to S_{q-1}(X)$ is a group homomorphism. We also define $\partial_q=0$ for $q\leq 0$ .

![《同调论》姜伯驹 P10](https://pic4.zhimg.com/80/v2-a590ed2fefa931d90e0abdb7ac9a77f3.jpg)

$\bf Rmk$

Note that $(e_0\dots\hat e_i\dots e_q):\Delta_{q-1}\to\Delta_q$ and $\sigma_q:\Delta_q\to X$ , therefore the right-hand side is an element of $S_{q-1}(X)$ .

<br/><br/>

$\bf Prop\ 3.5$

$\partial_{q-1}\partial_q=0$ , thus $S_\ast(X)=(S_q(X),\partial_q)$ is a chain complex.

> $\it Proof$
>  
> $$
> \begin{aligned}
> &\partial_{q-1}\partial_q(\sigma_q)\\
> =&\partial_{q-1}\left(\sum_{i=0}^q(-1)^i\sigma_q\circ(e_0\dots\hat e_i\dots e_q)\right)\\
> =&\sum_{i=0}^q(-1)^i\partial_{q-1}(\sigma_q\circ(e_0\dots\hat e_i\dots e_q))\\
> =&\sum_{i=0}^q(-1)^i\left(
> \sum_{j=0}^{i-1}(-1)^j\sigma_q(e_0\dots\hat e_j\dots\hat e_i\dots e_q)
> +\sum_{j=i+1}^{q}(-1)^j\sigma_q(e_0\dots\hat e_i\dots\hat e_j\dots e_q)
> \right)\\
> =&\sum_{i>j}(-1)^{i+j}\sigma_q(e_0\dots\hat e_j\dots\hat e_i\dots e_q)
> +\sum_{j>i}(-1)^{i+j-1}\sigma_q(e_0\dots\hat e_i\dots\hat e_j\dots e_q)=0
> \end{aligned}
> $$

$\bf Def\ 3.6\text{ (singular chain complex)}$

Chain complex $S_\ast(X)=(S_q(X),\partial_q)$ is called the singular chain complex of $X$ , whose homology groups are called the singular homology groups(奇异同调群) of $X$ , denoted by $H_\ast(X):=H_\ast(S_\ast(X))$ . The singular homology groups of negative dimension are all zeros $0$ .

<br/><br/>

$\bf Def\ 3.7\text{ (induced chain mapping)}$

A continuous map $f:X\to Y$ naturally induces homomorphisms $f_{\#}:S_\ast(X)\to S_\ast(Y)$ where $f_{\#q}(\sigma_q)=f\circ\sigma_q$ for any $\sigma_q:\Delta_q\to X$ . For any $c_q=\sum_{i=1}^r k_i\sigma_q^{(i)}\in S_q(X)$ , $f_{\#q}(c_q)=\sum_{i=1}^r k_if_{\#q}(\sigma_q^{(i)})$ .

$\bf Prop\ 3.8$

$f_{\#q-1}\partial_{q}=\partial_{q}f_{\#q}$ , thus $f_{\#}:S_\ast(X)\to S_\ast(Y)$ is a chain mapping.

> $\it Proof$
>  
> $$
> \begin{aligned}
> &f_{\#q-1}\partial_{q}(\sigma_q)\\
> =&f_{\#q-1}\left(\sum_{i=0}^q(-1)^i\sigma_q\circ(e_0\dots\hat e_i\dots e_q)\right)\\
> =&\sum_{i=0}^q(-1)^if_{\#q-1}(\sigma_q\circ(e_0\dots\hat e_i\dots e_q))\\
> =&\sum_{i=0}^q(-1)^if\circ \sigma_q\circ(e_0\dots\hat e_i\dots e_q)\\
> =&\partial_{q}(f\circ \sigma_q)
> =\partial_{q}(f_{\#q-1}(\sigma_q))
> =\partial_{q}f_{\#q-1}(\sigma_q)
> \end{aligned}
> $$

$\bf Rmk$

1. Given two mappings $f:X\to Y,g:Y\to Z$ , we have $(gf)_\#=g_\#f_\#$ ；
2. By the Rmk of Prop2.4, $(gf)_{\#\ast}=g_{\#\ast}f_{\#\ast}$ .

<br/><br/>

$\bf Thm\ 3.9$

Singular homology group is a topological invariant(同胚不变量). That is, if $f:X\to Y$ is a homeomorphism, then $f_{\#\ast}:H_\ast(X)\to H_\ast(Y)$ are group isomorphisms.

> $\it Proof$
>  
> Let $g=f^{-1}:Y\to X$ , then $g_{\#\ast}f_{\#\ast}=(gf)_{\#\ast}=\mathrm{id}_{\#\ast}=\mathrm{id}:H_\ast(Y)\to H_\ast(X)$ . Similarly we can prove $f_{\#\ast}g_{\#\ast}=\mathrm{id}:H_\ast(X)\to H_\ast(Y)$ . Therefore $f_{\#\ast}$ is bijective, hence isomorphic.

<br/><br/>

Now we are going to compute the homology groups of some spaces.

$\bf Prop\ 3.10\text{ (homology groups of a single point)}$

Use $\mathrm{pt}$ to represent a space of a single point, then $H_q(\mathrm{pt})\cong\begin{cases}\mathbb{Z}&q=0\\0&q\neq 0\end{cases}$

> $\it Proof$
>  
> Note that for any $q\geq0$ , there is a unique singular $q$-simplex $\sigma_q:\Delta_q\to\mathrm{pt}$ , we obtain that $S_q(\mathrm{pt})=\{k\sigma_q:k\in\mathbb{Z}\}\cong\mathbb{Z}$ . For any $q\geq1$ , $\partial_q(\sigma_q)=\sum_{i=0}^q(-1)^i\sigma_q\circ(e_0\dots\hat e_i\dots e_q)=\sum_{i=0}^q(-1)^i\sigma_{q-1}=\begin{cases}0&q\text{ is odd}\\\sigma_{q-1}&q\text{ is even}\end{cases}$ , thus $\partial_q=\begin{cases}0&q\text{ is odd}\\\mathrm{id}&q\text{ is even}\end{cases}$ . 
>  
> $$\begin{CD}
> S_\ast(\mathrm{pt}):\ \overset{3,odd}{\mathbb{Z}}
> @>0>> \overset{2,even}{\mathbb{Z}}
> @>\mathrm{id}>> \overset{1,odd}{\mathbb{Z}}
> @>0>> \overset{0}{\mathbb{Z}}
> @>0>> \overset{-1}0
> \end{CD}$$

<br/><br/>

There are many interesting properties of singular 0-simplex. 

Note that any singular 0-simplex $\sigma_0:\Delta_0\to X$ can be seen as a point in $X$ . For any singular 0-chain $c_0=k_1a_1+\dots+k_ra_r$ (Here $a_i$ are points in $X$), we define the **Kronecker index** of $c_0$ to be $\varepsilon(c_0)=k_1+\dots+k_r$ .

One can easily prove that $\varepsilon:S_0(X)\to\mathbb{Z}$ is a surjective homomorphism with $\mathrm{Im}(\varepsilon)=\mathbb{Z}$ , then by FHT we obtain $Z_0(X)/\mathrm{Ker}(\varepsilon)=S_0(X)/\mathrm{Ker}(\varepsilon)\cong\mathrm{Im}(\varepsilon)=\mathbb{Z}$ .

$\bf Thm\ 3.11$

$X$ is path-connected iff $H_0(X)\cong\mathbb{Z}$ .

> $\it Proof$
>  
> We first prove $(\Rightarrow)$ . It suffices to show $B_0(X)=\mathrm{Ker}(\varepsilon)$ , then $H_0(X)=Z_0(X)/B_0(X)=Z_0(X)/\mathrm{Ker}(\varepsilon)\cong\mathbb{Z}$ . It is obvious that $B_0(X)\subset\mathrm{Ker}(\varepsilon)$ . Now we try to show the opposite direction.
>  
> Take a point $b\in X$ as a base point. $\forall a\in X$ , there exists a path $\sigma:[0,1]\to X$ , which is actually a singular 1-simplex with $\partial\sigma=a-b$ , connecting $a$ and $b$ . That is, $a-b\in B_0(X)$ . Therefore $\forall c_0\in\mathrm{Ker}(\varepsilon)$ , we have $c_0=c_0-\varepsilon(c_0)b=\sum k_i(a_i-b)\in B_0(X)$ . So we obtain $\mathrm{Ker}(\varepsilon)\subset B_0(X)$ .

<br/><br/>

To prove $(\Leftarrow)$ , we need further preparations.

$\bf Def\ 3.12\text{ (direct sum of chain complexes)}$

The direct sum of a family of chain complexes $(C_\lambda,\partial_\lambda),\lambda\in\Lambda$ is $\bigoplus_{\lambda\in\Lambda}C_\lambda=\{\bigoplus_{\lambda\in\Lambda}C_\lambda,\bigoplus_{\lambda\in\Lambda}\partial_\lambda\}$ . One can prove by definition that $H_\ast(\bigoplus_{\lambda\in\Lambda}C_\lambda)=\bigoplus_{\lambda\in\Lambda}H_\ast(C_\lambda)$ .

$\bf Thm\ 3.13$

Assume $X=\bigcup_{\lambda\in\Lambda}X_\lambda$ where $X_\lambda$ are the path-connected components of $X$ , then $H_\ast(X)=\bigoplus_{\lambda\in\Lambda}H_\ast(X_\lambda)$ .

> $\it Proof$
>  
> Let $\Sigma_X$ be the set of all the singular simplices of $X$ . It's obvious that $\Sigma_X=\bigsqcup_{\lambda\in\Lambda}\Sigma_{X_\lambda}$ , hence $S_\ast(X)=\bigoplus_{\lambda\in\Lambda}S_\ast(X_\lambda)$ .

Therefore $H_0(X)\cong\mathbb{Z}$ implies that $X$ has only one path-connected component, thus path-connected.

<br/><br/>

### 3.3 Reduced singular homology group

$\bf Def\ 3.14\text{ (augment singular chain complex)}$

The augment singular chain complex(增广奇异链复形) of $X$ is $\widetilde S_\ast(X)=(\widetilde S_q(X),\widetilde \partial_q)$ where $\widetilde S_q(X)=\begin{cases}S_q(X)&q\neq-1\\\mathbb{Z}&q=-1\end{cases}$ and $\widetilde \partial_q=\begin{cases}\partial_q&q\neq0\\\varepsilon&q=0\end{cases}$ .

$\bf Def\ 3.15\text{ (reduced singular homology group)}$

The homology group of $\widetilde S_\ast(X)$ are called reduced singular homology groups(简约奇异同调群), denoted by $\widetilde H_\ast(X)$ . One can prove that $\widetilde H_q(X)=H_q(X)$ when $q\neq 0$ .

$\bf Thm\ 3.16$

$X$ is path-connected iff $\widetilde H_0(X)\cong 0$ .

<br/><br/>

A continuous map $f:X\to Y$ induces $f_\#0:S_0(X)\to S_0(Y)$ . Note that $\varepsilon(f_\#0(c_0))=\varepsilon(c_0)$ for any $c_0\in S_0(X)$ , we define $f_{\#-1}=\mathrm{id}:\mathbb{Z}\to\mathbb{Z}$ , then $f_\#$ is chain mapping between $\widetilde S_\ast(X)$ and $\widetilde S_\ast(Y)$ .

<br/><br/>

$\bf e.g.\text{ (reduced homology groups of a single point)}$

$\widetilde H_q(\mathrm{pt})=0$

<br/><br/>

$\bf e.g.\text{ (reduced homology groups of two points)}$

$A=\{a_0,a_1\}$ with discrete topology, then $\widetilde H_q(A)\cong\begin{cases}\mathbb{Z}&q=0\\0&q\neq 0\end{cases}$ and a generator of $\widetilde H_0(A)$ is $[a_1-a_0]$ , where $a_i:\Delta_0\to\{a_i\}$ are singular simplices . 

> $\it Proof$
>  
> $A$ has two path-connected components $\{a_0\}$ and $\{a_1\}$ , thus the reduced singular chain complex of $A$ is
>  
> $$\begin{CD}
> \widetilde S_\ast(A):\ \overset{3,odd}{\mathbb{Z}\oplus\mathbb{Z}}
> @>0>> \overset{2,even}{\mathbb{Z}\oplus\mathbb{Z}}
> @>\mathrm{id}>> \overset{1,odd}{\mathbb{Z}\oplus\mathbb{Z}}
> @>0>> \overset{0}{\mathbb{Z}\oplus\mathbb{Z}}
> @>\varepsilon>> \overset{-1}{\mathbb{Z}}
> \end{CD}$$
>  
> When $q=0$ , $\widetilde H_0(A)=\mathrm{Ker}(\varepsilon)/\mathrm{Im}(0)\cong\mathrm{Ker}(\varepsilon)\cong\mathbb{Z}$ .
>  
> $\forall c_0=k_0a_0+k_1a_1\in\mathrm{Ker}(\varepsilon)$ , $\varepsilon(c_0)=k_0+k_1=0$ , thus $c_0=k_1(a_1-a_0)$ . Therefore $[a_1-a_0]$ is a generator of $\widetilde H_0(A)$ .

<br/><br/>

### 3.4 Homotopic invariant property of homology groups

$\bf Thm\ 3.17$

Two homotopic continuous maps $f\simeq g:X\to Y$ induce chain homotopic chain mappings $f_\#\simeq g_\#:S_\ast(X)\to S_\ast(Y)$ . Therefore by Thm 2.6, they induce the same homology homomorphism $f_{\#\ast}=g_{\#\ast}:H_\ast(X)\to H_\ast(Y)$ .

> $\it Proof$
>  
> By condition, there exists a continuous map $F:X\times I\to Y$ such that $f(x)=F(x,0)$ and $g(x)=G(x,1)$ .For $i=0,1$ , let $c_i:X\to X\times I,x\mapsto(x,i)$ , then $f=F\circ c_0$ and $g=F\circ c_1$ . If we can prove $c_{0\#}\simeq c_{1\#}:S_\ast(X)\to S_\ast(X\times I)$ are chain homotopic, then it follows from Prop 2.8 that $f_\#=F_\#\circ c_{0\#}\simeq F_\#\circ c_{1\#}=g_\#$ .
>  
> To prove $c_{0\#}\simeq c_{1\#}:S_\ast(X)\to S_\ast(X\times I)$ , we need to construct $P:S_q(X)\to S_{q+1}(X\times I)$ such that $\partial\circ P+P\circ \partial=c_{1\#}-c_{0\#}$ .

The map $P:S_q(X)\to S_{q+1}(X\times I)$ mentioned above is actually dividing the cylinder(柱形) $\Delta_q\times I$ into several simplices $\Delta_{q+1}$ . Take $q=1$ and $q=2$ as an example.

![《同调论》姜伯驹 P15](https://pic4.zhimg.com/80/v2-d42986fe96f540d614635469dae47212.jpg)

To that effect, for any singular simplex $(e_0e_1\dots e_n):\Delta_q\to\Delta_q$ , we define the cylinder chain(柱形链) as $P(e_0e_1\dots e_n)=\sum_{i=0}^q(-1)^i(a_0\dots a_ib_i\dots b_q)\in S_{q+1}(\Delta_q\times I)$ where $a_i=e_i\times\{0\}$ and $b_i=e_i\times\{1\}$ .

$\bf Lemma\ 3.18\text{ (boundary formula of cylinder chain)}$

$\partial P(e_0\dots e_n)=(b_0\dots b_q)-(a_0\dots a_q)-\sum_{i=0}^q(-1)^iP(e_0\dots \hat e_i\dots e_n)$

<br/><br/>

> $\it End\ of\ proof\ of\ Thm\ 3.17$
>  
> For any singular simplex $\sigma_q:\Delta_q\to X$ , we define $P(\sigma_q)=(\sigma\times\mathrm{id})_\#(P(e_0\dots e_q))\in S_{q+1}(X\times I)$ . For any $c_q=\sum_{i=1}^nk_i\sigma^{(i)}_q\in S_q(X)$ , we define $P_q(c_q)=\sum_{i=1}^nk_iP(\sigma^{(i)}_q)$ . Then $P:S_q(X)\to S_{q+1}(X\times I)$ are homomorphisms.
>  
> $$\begin{aligned}
> \partial P(\sigma)&=(\sigma\times\mathrm{id})_\#(\partial P(e_0\dots e_q))\\
> &=(\sigma\times\mathrm{id})_\#\left((b_0\dots b_q)-(a_0\dots a_q)-\sum_{i=0}^q(-1)^iP(e_0\dots \hat e_i\dots e_n)\right)\\
> &=(\sigma\times\mathrm{id})_\#\left((e_0\dots e_q)\times\{0\}-(e_0\dots e_q)\times\{1\}-\sum_{i=0}^q(-1)^iP(e_0\dots \hat e_i\dots e_n)\right)\\
> &=c_{1\#}(\sigma)-c_{0\#}(\sigma)-P(\partial \sigma)
> \end{aligned}$$
>  
> $\partial\circ P+P\circ\partial=c_{1\#}-c_{0\#}$ , therefore $c_{0\#}\simeq c_{1\#}$ .

<br/><br/>

$\bf Cor\ 3.19$

Singular homology group is a homotopy invariant(同伦不变量). That is, if $X\simeq Y$ are homotopy equivalent, then $H_\ast(X)\cong H_\ast(Y)$ are isomorphism.

> $\it Proof$
>  
> $\exists f:X\to Y$ and $g:Y\to X$ such that $g\circ f\simeq\mathrm{id}_X$ and $f\circ g\simeq\mathrm{id}_Y$ . By Thm 3.17, $g\circ f\simeq\mathrm{id}_X\Rightarrow g_{\#\ast}\circ f_{\#\ast}=(g\circ f)_{\#\ast}=\mathrm{id}$ , symmetrically $f_{\#\ast}\circ g_{\#\ast}=\mathrm{id}$ . In terms of mapping, we obtain $f_{\#\ast}:H_\ast(X)\to H_\ast(Y)$ is bijective , thus isomorphic.

<br/><br/>

Recall:

$A\subset X$ is called a deformation retract((强)形变收缩核) from $X$ to $A$ if there exists a homotopy $G:X\times I\to X$ such that $G(x,0)=x$ , $G(x,1)\in A$ and $G(a,t)=a,\forall a\in A$ .

Assume $A$ is a deformation retract of $X$ . Take $r:X\to A,x\mapsto G(x,1)$ and inclusion map $i:A\to x$ , then $i\circ r:X\to X\overset{G}\simeq\mathrm{id}_X$ and $r\circ i:A\to A=\mathrm{id}_A\simeq\mathrm{id}_A$ , therefore $A$ and $X$ are homotopy equivalent. 

$\bf Cor\ 3.20$

If $A$ is a deformation retract of $X$ , then the inclusion map $i:A\to X$ induces $i_{\#\ast}:H_\ast(A)\cong H_\ast(X)$ .

<br/><br/>

### 3.6 $\mathscr{U}-$small singular chain

Assume $\mathscr{U}$ is a covering of $X$ , i.e. $X=\bigcup_{U\in\mathscr{U}}U$ . A singular simplex $\sigma:\Delta_q\to X$ is called $\mathscr{U}-$small if $\exist U\in\mathscr{U}$ such that $\sigma(\Delta_q)\subset U$ .

Let $S_q^\mathscr{U}(X)=\{\sum_{i=1}^r k_i\sigma_q^{(i)}:\sigma_q^{(i)}\text{ is }\mathscr{U}\text{-small}\}\subset S_q(X)$ , then $S_\ast^\mathscr{U}(X)=(S_q^\mathscr{U}(X),\partial_q)$ is a chain complex. The inclusion map $i:S_\ast^\mathscr{U}(X)\to S_\ast(X)$ is chain mapping , i.e. $i\circ\partial=\partial\circ i$ .

$\bf Thm\ 3.21$

If $\mathscr{U}$ is an open covering of $X$ , then $i:S_\ast^\mathscr{U}(X)\to S_\ast(X)$ is a chain chain homotopy equivalence, i.e. 